more reorganisations and cleanups around untyped conversion
guess who forgot there already was a proof of termination around that was not in the CoqProject and hadn't been updated for months?

theories/TypingProperties/Normalisation.v
@@ -185,7 +185,62 @@ Lemma dnf_whnf :
 Proof.
   apply DeepNormInduction.
   all: intros ; prod_splitter ; prod_hyp_splitter ;
-    try solve [eauto using isPosType_isType | econstructor ; eauto].
+    try solve [eauto using isPosType_isType, isFun_whnf, isPair_whnf | econstructor ; eauto].
+Qed.
+
+Lemma dnf_ren :
+  DeepNormInductionConcl
+  (fun (Γ : context) (A t : term) => forall Δ (ρ : Δ ≤ Γ), dnorm_tm Δ A⟨ρ⟩ t⟨ρ⟩)
+  (fun (Γ : context) (A t : term) => forall Δ (ρ : Δ ≤ Γ), dnf_tm Δ A⟨ρ⟩ t⟨ρ⟩)
+  (fun (Γ : context) (A t : term) => forall Δ (ρ : Δ ≤ Γ), dneu Δ A⟨ρ⟩ t⟨ρ⟩)
+  (fun (Γ : context) (A t : term) => forall Δ (ρ : Δ ≤ Γ), dneu_red Δ A⟨ρ⟩ t⟨ρ⟩)
+  (fun (Γ : context) (A : term) => forall Δ (ρ : Δ ≤ Γ), dnorm_ty Δ A⟨ρ⟩)
+  (fun (Γ : context) (A : term) => forall Δ (ρ : Δ ≤ Γ), dnf_ty Δ A⟨ρ⟩).
+Proof.
+  apply DeepNormInduction.
+  all: try (intros ; solve [now econstructor ; eauto using credalg_wk]).
+  all: try solve [econstructor ; eauto ; cbn ; now erewrite <- !wk_up_ren_on].
+  - intros * ?? IH **.
+    econstructor.
+    1: now apply whnf_ren.
+    epose proof (IH _ (wk_up _ _)) as IH' ; cbn in IH'.
+    assert (forall t, t⟨ρ⟩⟨↑⟩ = t⟨↑⟩⟨up_ren ρ⟩) as ->
+      by (now asimpl).
+    now rewrite wk_up_ren_on in IH'.
+  - econstructor ; eauto.
+    1: now apply whnf_ren.
+    erewrite <- wk_up_ren_on, wk_fst, <- subst_ren_wk_up; eauto.
+  - econstructor ; eauto.
+    now apply isPosType_ren.
+  - intros.
+    econstructor.
+    now eapply in_ctx_wk.
+  - intros.
+    erewrite subst_ren_wk_up.
+    econstructor ; eauto.
+    now rewrite wk_prod.
+  - intros.
+    erewrite subst_ren_wk_up.
+    econstructor ; eauto.
+    + now erewrite <- wk_up_ren_on.
+    + now erewrite <- (wk_up_ren_on _ _ _ tNat), <- (subst_ren_wk_up (n := tZero) ρ).
+    + now erewrite <- wk_up_ren_on, wk_elimSuccHypTy.
+  - intros.
+    erewrite subst_ren_wk_up.
+    econstructor ; eauto.
+  - intros.
+    erewrite subst_ren_wk_up.
+    econstructor ; eauto.
+    now rewrite wk_sig.
+  - intros * ?? ? IHP ? IHr **.
+    erewrite <- !wk_idElim, subst_ren_wk_up2.
+    econstructor ; eauto.
+    + now erewrite !wk_up_wk1.
+    + now rewrite wk_refl, <- subst_ren_wk_up2.
+  - econstructor ; eauto using credalg_wk.
+    now apply whnf_ren.
+    Unshelve.
+    all: assumption.
 Qed.
 
 Lemma dnf_det :
@@ -205,3 +260,231 @@ Proof.
   1-3: congruence.
   subst ; now eapply whred_det.
 Qed.
+
+
+
+(** Untyped deeply normalising terms *)
+Inductive udnorm : term -> Type :=
+| UDeepRed {t t'} :
+  [t ⤳* t'] ->
+  udnf t' ->
+  udnorm t
+(** Deep normal forms (whnf, recursively containing normalising subterms), untyped (no η-expansion) *)
+with udnf : term -> Type :=
+| UDeepU :
+    udnf U
+| UDeepPi {A B} :
+    udnorm A ->
+    udnorm B ->
+    udnf (tProd A B)
+| UDeepNat :
+    udnf tNat
+| UDeepZero :
+    udnf tZero
+| UDeepSucc {t} :
+    udnorm t ->
+    udnf (tSucc t)
+| UDeepEmpty :
+    udnf tEmpty
+| UDeepLam {A f} :
+    udnorm f ->
+    udnf (tLambda A f)
+| UDeepSig {A B} :
+    udnorm A ->
+    udnorm B ->
+    udnf (tSig A B)
+| UDeepPair {A B p q} :
+  udnorm p ->
+  udnorm q ->
+  udnf (tPair A B p q)
+| UDeepId {A x y} :
+  udnorm A ->
+  udnorm x ->
+  udnorm y ->
+  udnf (tId A x y)
+| UDeepRefl {A x} :
+  udnf (tRefl A x)
+| UDeepNeu {m} :
+  udneu m ->
+  udnf m
+(** Deep neutrals (wh neutrals, with recursively normalising/neutral subterms), untyped *)    
+with udneu : term -> Type :=
+| UDeepVar {n} :
+  udneu (tRel n)
+| neuUDeepApp {n t} :
+  udneu n ->
+  udnorm t ->
+  udneu (tApp n t)
+| neuUDeepNatElim {n P hz hs} :
+  udneu n ->
+  udnorm P ->
+  udnorm hz ->
+  udnorm hs ->
+  udneu (tNatElim P hz hs n)
+| neuUDeepEmptyElim {P n} :
+  udneu n ->
+  udnorm P ->
+  udneu (tEmptyElim P n)
+| neuUDeepFst {n} :
+  udneu n ->
+  udneu (tFst n)
+| neuUDeepSnd {n} :
+  udneu n ->
+  udneu (tSnd n)
+| neuUDeepIdElim {A x P hr y n} :
+  udneu n ->
+  udnorm P ->
+  udnorm hr ->
+  udneu (tIdElim A x P hr y n).
+
+Section InductionScheme.
+
+  Scheme 
+    Minimality for udnorm Sort Type with
+    Minimality for udnf   Sort Type with
+    Minimality for udneu     Sort Type.
+
+  Combined Scheme _UDeepNormInduction from
+      udnorm_rect_nodep,
+      udnf_rect_nodep,
+      udneu_rect_nodep.
+
+  Let _UDeepNormInductionType :=
+    ltac:(let ind := fresh "ind" in
+        pose (ind := _UDeepNormInduction);
+        refold ;
+        let ind_ty := type of ind in
+        exact ind_ty).
+
+  Let UDeepNormInductionType :=
+    ltac: (let ind := eval cbv delta [_UDeepNormInductionType] zeta
+      in _UDeepNormInductionType in
+      let ind' := polymorphise ind in
+    exact ind').
+
+  Lemma UDeepNormInduction : UDeepNormInductionType.
+  Proof.
+    intros PNorm PNf PNeu  **.
+    pose proof (_UDeepNormInduction PNorm PNf PNeu) as H.
+    destruct H as (?&?&?).
+    all: try (assumption ; fail).
+    repeat (split;[assumption|]); assumption.
+  Qed.
+
+  Definition UDeepNormInductionConcl :=
+    ltac:(
+      let t := eval cbv delta [UDeepNormInductionType] beta in UDeepNormInductionType in
+      let t' := remove_steps t in
+      exact t').
+
+End InductionScheme.
+
+Section DeepUDeep.
+
+  Lemma udeep_ren :
+  UDeepNormInductionConcl
+    (fun t => forall ρ, udnorm t⟨ρ⟩)
+    (fun t => forall ρ, udnf t⟨ρ⟩)
+    (fun t => forall ρ, udneu t⟨ρ⟩).
+  Proof.
+    apply UDeepNormInduction.
+    all: try solve [econstructor ; eauto].
+    intros * Hred **.
+    econstructor.
+    1: now eapply credalg_wk in Hred.
+    eauto.
+  Qed.
+
+  Lemma udnf_whnf :
+    UDeepNormInductionConcl
+    (fun _ => True)
+    (fun t => whnf t)
+    (fun t => whne t).
+  Proof.
+    apply UDeepNormInduction.
+    all: intros ; prod_splitter ; prod_hyp_splitter ;
+      try solve [eauto using isPosType_isType, isFun_whnf, isPair_whnf | econstructor ; eauto].
+  Qed.
+
+  Lemma udeep_exp t t' : udnorm t -> [t' ⤳* t] -> udnorm t'.
+  Proof.
+    intros Hnorm ?.
+    inversion Hnorm ; subst.
+    econstructor ; [|eassumption].
+    now etransitivity.
+  Qed.
+
+  Lemma udeep_red t t' : udnorm t -> [t ⤳* t'] -> udnorm t'.
+  Proof.
+    intros Hnorm ?.
+    inversion Hnorm ; subst.
+    econstructor ; [|eassumption].
+    eapply whred_red_det ; tea.
+    now apply udnf_whnf.
+  Qed.
+
+  (* Lemma deep_udeep :
+    DeepNormInductionConcl
+      (fun _ _ t => (udnorm t) × (whne t -> udneu t))
+      (fun _ _ t => (udnf t) × (whne t -> udneu t))
+      (fun _ _ t => udneu t)
+      (fun _ _ t => udneu t)
+      (fun _ t => (udnorm t) × (whne t -> udneu t))
+      (fun _ t => (udnf t) × (whne t -> udneu t)).
+  Proof.
+    apply DeepNormInduction.
+    all: try (intros ; try split ; intros ; solve
+      [easy | now econstructor | match goal with | Hne : whne _ |- _ => inversion Hne end]).
+    - intros ? t t' **.
+      prod_hyp_splitter ; split ; intros.
+      1: now econstructor.
+      enough (t = t') as -> by easy.
+      apply red_whnf ; gen_typing.
+    - intros ? f * Hfun Hnf [? Hne].
+      assert (whne f -> udneu f).
+      {
+        intros.
+        assert (whne (eta_expand f)) as Hexp by (constructor ; now eapply whne_ren).
+        specialize (Hne Hexp).
+        inversion Hne ; subst.
+        erewrite <- (wk_section (wk1 _)).
+        eapply udeep_ren.
+        now erewrite wk1_ren_on.
+        Unshelve.
+        all: eassumption.
+      }
+      split ; [..|easy].
+      destruct Hfun ; [|now constructor].
+      constructor.
+      eapply udeep_red.
+      1: eassumption.
+      econstructor ; eauto using eta_expand_beta ; reflexivity.
+    - intros * Hpair Hnf [IHf Hne] ? [IHs].
+      assert (whne p -> udneu p).
+      {
+        intros.
+        specialize (Hne ltac:(gen_typing)).
+        now inversion Hne.
+      }
+      split ; [..|easy].
+      destruct Hpair ; [..|now econstructor].
+      constructor ; eauto.
+      + eapply udeep_red.
+        1: eapply IHf.
+        econstructor.
+        1: now econstructor.
+        reflexivity.
+      + eapply udeep_red.
+        1: eapply IHs.
+        econstructor.
+        1: now econstructor.
+        reflexivity.
+    - intros * ? ? [].
+      split.
+      1: now econstructor.
+      intros.
+      enough (A = A') as -> by easy.
+      now eapply red_whne.
+  Qed. *)
+
+End DeepUDeep.
