theories/Algorithmic/AlgorithmicTypingProperties.v
@@ -5,7 +5,7 @@ From LogRel.Algorithmic Require Import BundledAlgorithmicTyping AlgorithmicConvP
 
 From LogRel Require Import Utils.
 
-Import DeclarativeTypingProperties AlgorithmicTypingData BundledTypingData.
+Import DeclarativeTypingProperties AlgorithmicTypingData.
 
 (** ** Small types are large types *)
 
@@ -14,37 +14,146 @@ while in the definition of algorithmic typing we only allow it when A is a non-c
 type (in which case it has to be small).
 So we need to show admissibility of the more general rule. *)
 
-Lemma algo_typing_small_large
-  `{!TypingSubst de} `{!TypeReductionComplete de} `{!TypeConstructorsInj de}
-  Γ A :
-  [Γ |-[bn] A : U] ->
-  [Γ |-[bn] A].
-Proof.
-  enough (BundledTypingInductionConcl
-    (fun _ _ => True)
-    (fun Γ A t => [Γ |-[de] A ≅ U] -> [Γ |-[al] t])
-    (fun Γ A t => A = U -> [Γ |-[al] t])
-    (fun _ _ _ => True)) as (?&?&H&?).
-  {
-    intros [].
-    split ; tea.
-    eapply H.
-    2: reflexivity.
-    do 2 (econstructor ; tea).
-    now eapply redty_red, red_compl_univ_r.
-    constructor.
-  }
-  eapply BundledTypingInduction.
-  all: try solve [
-    econstructor |
-    intros; econstructor; [intros Hcan; inversion Hcan| econstructor;[now econstructor|now eapply redty_red, red_compl_univ_r|constructor]]|
-    intros; match goal with H : [_ |- _ ≅ _] |- _ => unshelve eapply ty_conv_inj in H; try now econstructor; now cbn in H end ].
+Section SmallLarge.
+  Import AlgorithmicTypedConvData BundledTypingData.
+  Context `{!TypingSubst de} `{!TypeReductionComplete de} `{!TypeConstructorsInj de}.
 
-    intros * ? [IH []] **; subst.
-    eapply IH.
-    eapply subject_reduction_type ; tea.
-    boundary.
-Qed.
+  Lemma algo_typing_small_large Γ A :
+    [Γ |-[bn] A : U] ->
+    [Γ |-[bn] A].
+  Proof.
+    enough (BundledTypingInductionConcl
+      (fun _ _ => True)
+      (fun Γ A t => [Γ |-[de] A ≅ U] -> [Γ |-[al] t])
+      (fun Γ A t => A = U -> [Γ |-[al] t])
+      (fun _ _ _ => True)) as (?&?&H&?).
+    {
+      intros [].
+      split ; tea.
+      eapply H.
+      2: reflexivity.
+      do 2 (econstructor ; tea).
+      now eapply redty_red, red_compl_univ_r.
+      constructor.
+    }
+    eapply BundledTypingInduction.
+    all: try solve [
+      econstructor |
+      intros; econstructor; [intros Hcan; inversion Hcan| econstructor;[now econstructor|now eapply redty_red, red_compl_univ_r|constructor]]|
+      intros; match goal with H : [_ |- _ ≅ _] |- _ => unshelve eapply ty_conv_inj in H; try now econstructor; now cbn in H end ].
+
+      intros * ? [IH []] **; subst.
+      eapply IH.
+      eapply subject_reduction_type ; tea.
+      boundary.
+  Qed.
+
+End SmallLarge.
+
+(** The shape of the inferred type is the same as that of any type *)
+
+Section InferShape.
+  Import AlgorithmicTypingData.
+  Context `{ta : tag} `{! ConvType ta}.
+  Context `{!TypingSubst de} `{!TypeConstructorsInj de}.
+
+  Hypothesis conv_sound :
+    forall Γ A A', [Γ |-[de] A] -> [Γ |-[de] A'] -> [Γ |-[ta] A ≅ A'] -> [Γ |-[de] A ≅ A'].
+
+  Lemma infer_U Γ A T : [Γ |-[de] A : U] -> [Γ |-[ta] A ▹h T] -> T = U.
+  Proof.
+    intros Hde [Hal Hal']%dup.
+    eapply algo_infer_unique in Hal ; tea.
+    2: boundary.
+    assert (isType T).
+    {
+      eapply type_isType.
+      1: boundary.
+      now inversion Hal'.
+    }
+    unshelve eapply ty_conv_inj in Hal ; tea.
+    1: constructor.
+    destruct H ; cbn in * ; try easy.
+    now destruct s.
+  Qed.
+
+  Lemma infer_nat Γ A T : [Γ |-[de] A : tNat] -> [Γ |-[ta] A ▹h T] -> T = tNat.
+  Proof.
+    intros Hde [Hal Hal']%dup.
+    eapply algo_infer_unique in Hal ; tea.
+    2: boundary.
+    assert (isType T).
+    {
+      eapply type_isType.
+      1: boundary.
+      now inversion Hal'.
+    }
+    unshelve eapply ty_conv_inj in Hal ; tea.
+    1: constructor.
+    now destruct H ; cbn in *.
+  Qed.
+
+  Lemma infer_empty Γ A T : [Γ |-[de] A : tEmpty] -> [Γ |-[ta] A ▹h T] -> T = tEmpty.
+  Proof.
+    intros Hde [Hal Hal']%dup.
+    eapply algo_infer_unique in Hal ; tea.
+    2: boundary.
+    assert (isType T).
+    {
+      eapply type_isType.
+      1: boundary.
+      now inversion Hal'.
+    }
+    unshelve eapply ty_conv_inj in Hal ; tea.
+    1: constructor.
+    now destruct H ; cbn in *.
+  Qed.
+
+  Lemma infer_prod Γ A B f T : [Γ |-[de] f : tProd A B] -> [Γ |-[ta] f ▹h T] ->
+    ∑ A' B', T = tProd A' B'.
+  Proof.
+    intros Hde [Hal Hal']%dup.
+    eapply algo_infer_unique in Hal ; tea.
+    2: boundary.
+    assert (isType T).
+    {
+      eapply type_isType.
+      1: boundary.
+      now inversion Hal'.
+    }
+    unshelve eapply ty_conv_inj in Hal ; tea.
+    1: constructor.
+    destruct H ; cbn in * ; easy.
+  Qed.
+
+  Lemma infer_sig Γ A B f T : [Γ |-[de] f : tSig A B] -> [Γ |-[ta] f ▹h T] ->
+    ∑ A' B', T = tSig A' B'.
+  Proof.
+    intros Hde [Hal Hal']%dup.
+    eapply algo_infer_unique in Hal ; tea.
+    2: boundary.
+    assert (isType T).
+    {
+      eapply type_isType.
+      1: boundary.
+      now inversion Hal'.
+    }
+    unshelve eapply ty_conv_inj in Hal ; tea.
+    1: constructor.
+    destruct H ; cbn in * ; easy.
+  Qed.
+
+  Lemma infer_U_ty Γ A T : [Γ |-[de] A] -> [Γ |-[ta] A ▹h T] -> T = U.
+  Proof.
+    intros Hde Hal.
+    inversion Hde ; subst ; refold.
+    1-6: inversion Hal as [???? Hal'] ; subst ; refold.
+    1-6: inversion Hal' ; subst ; refold.
+    1-5: symmetry ; eapply red_whnf ; tea ; constructor.
+    now eapply infer_U.
+  Qed.
+
+End InferShape.
 
 Import BundledIntermediateData IntermediateTypingProperties.
 
@@ -53,6 +162,7 @@ Import BundledIntermediateData IntermediateTypingProperties.
 we easily derive our third instance. *)
 
 Module AlgorithmicTypingProperties.
+  Import AlgorithmicTypedConvData.
   Export BundledTypingData AlgorithmicConvProperties.
 
   #[local] Ltac intros_bn :=
@@ -76,7 +186,7 @@ Module AlgorithmicTypingProperties.
   Proof.
     all: cycle -1.
     1: intros; now eapply algo_typing_small_large.
-    1: intros_bn; now eapply algo_typing_wk.
+    1: intros_bn; eapply algo_typing_wk ; tea ; intros ; now eapply algo_conv_wk.
     1-3: intros_bn; now econstructor.
     intros_bn; econstructor; tea; econstructor ; tea; now eapply ty_conv_compl.
   Qed.
@@ -86,7 +196,7 @@ Module AlgorithmicTypingProperties.
     TypingProperties (ta := bn) := {}.
   Proof.
     - intros_bn.
-      + now eapply algo_typing_wk.
+      + now eapply algo_typing_wk; tea ; intros ; now eapply algo_conv_wk.
       + gen_typing.
     - intros_bn.
       + now econstructor.
@@ -214,7 +324,7 @@ Module AlgorithmicTypingProperties.
     - intros_bn.
       2: now apply credalg_wk.
       econstructor ; tea.
-      1: now eapply algo_typing_wk.
+      1: now eapply algo_typing_wk; tea ; intros ; now eapply algo_conv_wk.
       now eapply typing_wk.
     - intros * [? []]; assumption.
     - now intros * [].
@@ -391,7 +501,7 @@ Module AlgorithmicTypingProperties.
     RedTypeProperties (ta := bn) := {}.
   Proof.
     - intros_bn.
-      1: now apply algo_typing_wk.
+      1: now apply algo_typing_wk; tea ; intros ; now eapply algo_conv_wk.
       now apply credalg_wk.
     - intros * []; assumption.
     - now intros_bn.
@@ -415,7 +525,7 @@ Import AlgorithmicTypingData AlgorithmicTypingProperties.
 
 (** *** Uniqueness of types *)
 
-Lemma type_uniqueness `{! TypingImplies (ta := de) (ta' := bn)} Γ A A' t :
+Lemma type_uniqueness `{! TypingImplies de bn} Γ A A' t :
   [Γ |-[de] t : A] ->
   [Γ |-[de] t : A'] ->
   [Γ |-[de] A ≅ A'].
